#ä¸å®šç§¯åˆ†
##æœ‰ç†å‡½æ•°ç§¯åˆ†

$\displaystyle \int \frac{1+x^4}{1+x^6}dx$
**ğŸ§ å®Œå…¨å¹³æ–¹åå‡‘æ·»é¡¹ï¼Œå†ç”¨åˆ†éƒ¨ç§¯åˆ†ï¼Œæœ€åä¸€æ­¥éœ€è¦å°†åˆ†æ¯ç›¸ä¹˜å¾—å‡º$1+x^6$å†å‡‘å¾®åˆ†**
$=\displaystyle  \int \frac{1+x^4}{(1+x^2)(1-x^2+x^4)}dx$
$=\displaystyle  \int \frac{1-x^2+x^4+x^2}{(1+x^2)(1-x^2+x^4)}dx$
$=\displaystyle \int \frac{1+x^2-1}{(1+x^2)}dx+\int \frac{x^2}{1+x^6}dx$
$=x-\arctan x + \frac{1}{3}\arctan x^3 +C$

****
#å®šç§¯åˆ†
##æ±‚è§£å«å®šç§¯åˆ†å·çš„å‡½æ•°æ–¹ç¨‹
**è®¾$f(x)=3x^2-2 \displaystyle \int_0^1 f(x)dx$ï¼Œæ±‚$\displaystyle \int_1^2dx$**
**ğŸ§ å…ˆæ±‚å‡º$f(x)$ç„¶ååœ¨$[1,2]$ä¸Šç§¯åˆ†**
**è§£ï¼š** ä»¤$\displaystyle \int_0^1f(x)dx=A$ï¼Œä¸¤è¾¹åŒæ—¶åœ¨$[0,1]$ç§¯åˆ†

$\qquad$ $\displaystyle \int_0^1f(x)dx=3\int_0^1x^2dx-2A\int_0^1dx$

$\qquad$ $\rightarrow A=-1\qquad \therefore f(x)=3x^2-2$,ä¸¤è¾¹åœ¨$[1,2]$ç§¯åˆ†

$\qquad$ $\displaystyle  \int_1^2f(x)=3\int_1^2x^2-2\int _1^2dx$

$\qquad$ $\therefore \displaystyle \int_1^2f(x)=5$
****

**è®¾$\displaystyle  f(x)=3x-\sqrt{1-x^2}\int_0^1f^2(x)dx$æ±‚$f(x)$**
**ğŸ§ ä¸¤è¾¹åŒæ—¶å¹³æ–¹è®¾Aã€‚**
**è§£ï¼š** ä¸¤è¾¹åŒæ—¶å¹³æ–¹
$\qquad \displaystyle f^2(x)=9x^2-6x\sqrt{1-x^2}\int_0^1f^2(x)dx+(1-x^2)(\int_0^1f^2(x)dx)^2$

$\qquad $è®¾$\displaystyle \int_0^1f^2(x)dx=A \rightarrow A=3$æˆ–$\displaystyle A=\frac{3}{2}$

$\qquad$$\therefore \displaystyle f(x)=3x-3\sqrt{1-x^2} $æˆ–$\displaystyle f(x)=3x-\frac{3}{2}\sqrt{1-x^2}$

****
**è®¾$\displaystyle f(x)=x^2-x\int_0^2f(x)dx+2\int_0^1f(x)dx$,æ±‚$f(x)$**
**ğŸ§ åˆ†åˆ«è®¾ABï¼Œåˆ†åˆ«ç§¯åˆ†è”ç«‹æ–¹ç¨‹ç»„ã€‚**
**è§£ï¼š** è®¾$\displaystyle A=\int_0^2 f(x)dx\qquad B=\int_0^1f(x)dx$

$\qquad$ç­‰å¼åˆ†åˆ«åœ¨$[0,1]$å’Œ$[0,2]$ä¸Šç§¯åˆ†ï¼Œè”ç«‹æ–¹ç¨‹ç»„ã€‚
$\qquad$$\begin{cases}
    \displaystyle A=\int_0^2x^2dx+A\int_0^2xdx+2B\int_0^2dx   \\
    \displaystyle B=\int_0^1x^2dx+A\int_0^1xdx+2B\int_0^1dx
\end{cases}$
$\qquad$è§£å¾—$\displaystyle A=\frac{4}{3}\qquad B=\frac{1}{3}$
$\qquad \displaystyle \therefore f(x)=x^2-\frac{4}{3}x+\frac{2}{3} $

***
